Iris/Iris/Examples.lean
@@ -5,4 +5,6 @@ public import Iris.Examples.Namesets
 public import Iris.Examples.Proofs
 public import Iris.Examples.Resources
 public import Iris.Examples.HeapLang
+public import Iris.Examples.LinkedList
+public import Iris.Examples.DoublyLinkedList
 public import Iris.Examples.ClosedProofs
